@prefix foaf: <http://xmlns.com/foaf/0.1/> .
@prefix schema: <http://schema.org/> .

@prefix owl: <http://www.w3.org/2002/07/owl#> .
@prefix rdfs: <http://www.w3.org/2000/01/rdf-schema#>.
@prefix pwd: <http://www.paasword.eu/security-policy/seerc/pwd#>.
@prefix otp: <http://www.paasword.eu/security-policy/seerc/otp#>.
@prefix pbe: <http://www.paasword.eu/security-policy/seerc/pbe#>.
@prefix pbdfd: <http://www.paasword.eu/security-policy/seerc/pbdfd#>.
@prefix pac: <http://www.paasword.eu/security-policy/seerc/pac#>.
@prefix rdf: <http://www.w3.org/1999/02/22-rdf-syntax-ns#>.
@prefix usdl-core: <http://www.linked-usdl.org/ns/usdl-core#>.
@prefix usdl-business-roles: <http://www.linked-usdl.org/ns/usdl-business-roles#>.
@prefix usdl-sec: <http://www.linked-usdl.org/ns/usdl-sec#>.
@prefix orgX: <http://www.paasword.eu/security-policy/orgX#>. 
@prefix gr: <http://purl.org/goodrelations/v1#>. 
@prefix pcm: <http://www.paasword-project.eu/ontologies/casm/2016/05/20#> .
@prefix pdm: <http://www.paasword-project.eu/ontologies/dsm/2016/05/20#> .
@prefix skos: <http://www.w3.org/2004/02/skos/core#> .
@prefix ppm: <http://www.paasword-project.eu/ontologies/psm/2016/05/20#> .
@prefix pcpm: <http://www.paasword-project.eu/ontologies/cpsm/2016/05/20#> .
@prefix xsd: <http://www.w3.org/2001/XMLSchema#>.

#
# PaaSword Permissions Model (version 2016-05-20)
# Some statements have been transferred to the constraints' ontology.
#
schema:Action a rdfs:Class .
ppm:DDLPermission
  a rdfs:Class ;
  rdfs:subClassOf ppm:Permission ;
  rdfs:comment "This class reveals the data definition language (DDL) related actions on specific objects." .

ppm:DataPermission
  a rdfs:Class ;
  rdfs:subClassOf schema:Action, ppm:Permission ;
  rdfs:comment "This is a class that describes any action allowed by a direct agent upon a data entity." .

ppm:DatastoreDDLPermission
  a rdfs:Class ;
  rdfs:subClassOf ppm:DDLPermission .

ppm:DatastorePermission
  a rdfs:Class ;
  rdfs:subClassOf ppm:DataPermission ;
  rdfs:comment "This is a class that describes any action allowed by a direct agent upon a data entity in a datastore." .

ppm:FilePermission
  a rdfs:Class ;
  rdfs:subClassOf ppm:DataPermission ;
  rdfs:comment "This is a class that describes any action allowed by a direct agent upon a file." .

ppm:FileSystemStructurePermission
  a rdfs:Class ;
  rdfs:subClassOf ppm:DDLPermission .

ppm:Permission
  a rdfs:Class ;
  rdfs:comment "This class refers to allowed actions of a subject upon an object." .

ppm:VolumePermission
  a rdfs:Class ;
  rdfs:subClassOf ppm:DataPermission .

ppm:WebEndpointPermission
  a rdfs:Class ;
  rdfs:subClassOf ppm:DataPermission ;
  rdfs:comment "This is a class that describes any Web endpoint action allowed by a direct agent upon a data entity in a datastore." .
#############################################################################