@prefix foaf: <http://xmlns.com/foaf/0.1/> .
@prefix schema: <http://schema.org/> .

@prefix owl: <http://www.w3.org/2002/07/owl#> .
@prefix rdfs: <http://www.w3.org/2000/01/rdf-schema#>.
@prefix pwd: <http://www.paasword.eu/security-policy/seerc/pwd#>.
@prefix otp: <http://www.paasword.eu/security-policy/seerc/otp#>.
@prefix pbe: <http://www.paasword.eu/security-policy/seerc/pbe#>.
@prefix pbdfd: <http://www.paasword.eu/security-policy/seerc/pbdfd#>.
@prefix pac: <http://www.paasword.eu/security-policy/seerc/pac#>.
@prefix rdf: <http://www.w3.org/1999/02/22-rdf-syntax-ns#>.
@prefix usdl-core: <http://www.linked-usdl.org/ns/usdl-core#>.
@prefix usdl-business-roles: <http://www.linked-usdl.org/ns/usdl-business-roles#>.
@prefix usdl-sec: <http://www.linked-usdl.org/ns/usdl-sec#>.
@prefix orgX: <http://www.paasword.eu/security-policy/orgX#>. 
@prefix gr: <http://purl.org/goodrelations/v1#>. 
@prefix pcm: <http://www.paasword-project.eu/ontologies/casm/2016/05/20#> .
@prefix pdm: <http://www.paasword-project.eu/ontologies/dsm/2016/05/20#> .
@prefix skos: <http://www.w3.org/2004/02/skos/core#> .
@prefix ppm: <http://www.paasword-project.eu/ontologies/psm/2016/05/20#> .
@prefix pcpm: <http://www.paasword-project.eu/ontologies/cpsm/2016/05/20#> .
@prefix xsd: <http://www.w3.org/2001/XMLSchema#>.

#
# PaaSword Data Distribution and Encryption Model (version 2016-05-20)
# Some statements have been transferred to the constraints' ontology.
#
pdm:Asymmetric
  a rdfs:Class ;
  rdfs:subClassOf pdm:CryptographicType ;
  rdfs:comment "Refers to the details of algorithm for cryptography chosen that uses the different cryptographic keys for  encryption (public key) of plaintext and decryption of ciphertext (private key)." .

pdm:CryptographicType
  a rdfs:Class ;
  rdfs:subClassOf pdm:DDEElement ;
  rdfs:comment "This class reveals details of the level of security required for specific sensitive data artefacts." .

pdm:DDEElement
  a rdfs:Class ;
  rdfs:comment "Parent class of all PaaSword Data Distribution and Encryption Model elements" .

pdm:DataDistribution
  a rdfs:Class ;
  rdfs:subClassOf pdm:DDEElement ;
  rdfs:comment "This class captures aspects of the data distribution  required for enhancing the security of sensitive information." .

pdm:DatabaseFragmentation
  a rdfs:Class ;
  rdfs:subClassOf pdm:DDEElement ;
  rdfs:comment "This class refers to the details concerning the way that the data should be fragmented in order to be distributed for security purposes." .

pdm:DistributionMetric
  a rdfs:Class ;
  rdfs:subClassOf pdm:DataDistribution ;
  rdfs:comment "This class quantifies the data distribution required for enhancing the security of sensitive information." .

pdm:ExcludedLocation
  a rdfs:Class ;
  rdfs:subClassOf pdm:DataDistribution ;
  rdfs:comment "This class denotes the physical locations that should be avoided when distributing sensitive data." .

pdm:ExcludedProvider
  a rdfs:Class ;
  rdfs:subClassOf pdm:DataDistribution ;
  rdfs:comment "This class denotes certain untrusted IaaS providers that should be avoided when distributing sensitive data." .

pdm:HorizontalFragmentation
  a rdfs:Class ;
  rdfs:subClassOf pdm:RelationalDataFragmentation ;
  rdfs:comment "This class refers to the fragmentation of a relational database across its rows." .

pdm:Hybrid
  a rdfs:Class ;
  rdfs:subClassOf pdm:Asymmetric, pdm:Symmetric .

pdm:MasterSlaveReplication
  a rdfs:Class ;
  rdfs:subClassOf pdm:Replication ;
  rdfs:comment "Master-slave replication refers into the details of making one node the authoritative copy that handles writes while slaves synchronizing with the master and handling reads." .

pdm:MixedFragmentation
  a rdfs:Class ;
  rdfs:subClassOf pdm:RelationalDataFragmentation ;
  rdfs:comment "This class refers to a two step  fragmentation process of a relational database that may use both horizontal and vertical fragmentation based on certain conditions." .

pdm:NonRelationalDataFragmentation
  a rdfs:Class ;
  rdfs:subClassOf pdm:DatabaseFragmentation ;
  rdfs:comment "This Class refers to different types of possible fragmentation of a non- relational database." .

pdm:PeerToPeerReplication
  a rdfs:Class ;
  rdfs:subClassOf pdm:Replication ;
  rdfs:comment "Peer-to-peer refers to the details of replication that allows writes to several nodes and synchronization between them." .

pdm:PreferredLocation
  a rdfs:Class ;
  rdfs:subClassOf pdm:DataDistribution ;
  rdfs:comment "This class denotes the physical locations that should be considered when distributing sensitive data." .

pdm:PreferredProvider
  a rdfs:Class ;
  rdfs:subClassOf pdm:DataDistribution ;
  rdfs:comment "This class denotes certain trusted IaaS providers that should be considered when distributing sensitive data." .

pdm:RelationalDataFragmentation
  a rdfs:Class ;
  rdfs:subClassOf pdm:DatabaseFragmentation ;
  rdfs:comment "This Class refers to different types of possible fragmentation of a relational database." .

pdm:Replication
  a rdfs:Class ;
  rdfs:subClassOf pdm:NonRelationalDataFragmentation ;
  rdfs:comment "Replication class refers to the details of copying data/aggregates across multiple servers, so each bit of data can be found in multiple places." .

pdm:Sharding
  a rdfs:Class ;
  rdfs:subClassOf pdm:NonRelationalDataFragmentation ;
  rdfs:comment "Sharding class refers to the details of  different data distribution across multiple servers, so each server acts as the single source for a subset of data/aggregates." .

pdm:Symmetric
  a rdfs:Class ;
  rdfs:subClassOf pdm:CryptographicType ;
  rdfs:comment "Refers to the details of algorithm for cryptography chosen that uses the same cryptographic keys for both encryption of plaintext and decryption of ciphertext." .

pdm:VerticalFragmentation
  a rdfs:Class ;
  rdfs:subClassOf pdm:RelationalDataFragmentation ;
  rdfs:comment "This class refers to the fragmentation of a relational database across its columns." .
#############################################################################